Finish a first working version of divDefLib.sml

backends/hol4/divDefLib.sml
@@ -15,30 +15,21 @@ raw_def_thm -> raw_def
 fuel_defs_thm -> fuel_defs (and split the theorem)
 *)
 
-(* TotalDefn.Define *)
-
-(*
-Datatype:
-  list_t =
-    ListCons 't list_t
-  | ListNil
-End
-*)
-
 (* TODO: move *)
 fun list_mk_arrow (tys : hol_type list) (ret_ty : hol_type) : hol_type =
   foldr (fn (ty, aty) => ty --> aty) ret_ty tys
 
-(*“test (x : bool) = (x <> F)” *)
-
+(*
 val def_qt = ‘
   (even (i : int) : bool result =
     if i = 0 then Return T else odd (i - 1)) /\
   (odd (i : int) : bool result =
     if i = 0 then Return F else even (i - 1))
 ’
+
 val def_tms = (strip_conj o list_mk_conj o rev) (Defn.parse_quote def_qt)
 val def_tm = hd def_tms
+*)
 
 (* Small utilities *)
 val current_goal : term option ref = ref NONE
@@ -87,10 +78,13 @@ val fuel_var1 = mk_var ("$m", “:num”) (* TODO: name collisions *)
 val fuel_vars_le = “^fuel_var0 <= ^fuel_var1”
 
 val fuel_predicate_suffix = "___P" (* TODO: name collisions *)
+val expand_suffix = "___E" (* TODO: name collisions *)
 
 val bool_ty = “:bool”
 
 val alpha_tyvar : hol_type = “:'a”
+val beta_tyvar : hol_type = “:'b”
+
 val is_diverge_def = Define ‘
   is_diverge (r: 'a result) : bool = case r of Diverge => T | _ => F’
 val is_diverge_tm = “is_diverge: 'a result -> bool”
@@ -101,6 +95,8 @@ val le_tm = (fst o strip_comb) “x:num <= y:num”
 val true_tm = “T”
 val false_tm = “F”
 
+val measure_tm = “measure: ('a -> num) -> 'a -> 'a -> bool”
+
 fun mk_diverge_tm (ty : hol_type) : term =
   let
     val diverge_ty = mk_thy_type {Thy="primitives", Tyop="result", Args = [ty] }
@@ -109,6 +105,143 @@ fun mk_diverge_tm (ty : hol_type) : term =
     diverge_tm
   end
 
+(*
+(* TODO: move *)
+fun strip_pair_type (ty : hol_type) : hol_type list =
+  let
+    val {Args=args, Thy=thy, Tyop=tyop} = dest_thy_type ty
+  in
+    if thy = "pair" andalso tyop = "prod" then
+      case args of
+        [x, y] => x :: strip_pair_type y
+      | _ => failwith "Unexpected"
+    else [ty]
+  end
+  handle HOL_ERR _ => [ty]
+
+fun list_mk_pair_type (tys : hol_type list) : hol_type =
+  case tys of
+    [] => failwith "Unexpected"
+  | [x] => x
+  | x :: tys =>
+    mk_thy_type {Args = [x, list_mk_pair_type tys], Thy="pair", Tyop="prod"}
+
+fun strip_sum_type (ty : hol_type) : hol_type list =
+  let
+    val {Args=args, Thy=thy, Tyop=tyop} = dest_thy_type ty
+  in
+    if thy = "sum" andalso tyop = "sum" then
+      case args of
+        [x, y] => x :: strip_sum_type y
+      | _ => failwith "Unexpected"
+    else [ty]
+  end
+  handle HOL_ERR _ => [ty]
+
+fun list_mk_sum_type (tys : hol_type list) : hol_type =
+  case tys of
+    [] => failwith "Unexpected"
+  | [x] => x
+  | x :: tys =>
+    mk_thy_type {Args = [x, list_mk_sum_type tys], Thy="sum", Tyop="sum"}
+*)
+
+
+(*
+val ty = “: ('a # 'b) # num # int”
+strip_pair_type ty
+list_mk_pair_type (strip_pair_type ty)
+
+val ty = “: ('a + 'b) + num + int”
+strip_sum_type ty
+list_mk_sum_type (strip_sum_type ty)
+
+val ty = “: (num # 'a # bool) + (num # int # bool) + (num # 'a)”
+*)
+
+(* Small utility: we sometimes need to generate a termination measure for
+   the fuel definitions.
+
+   We derive a measure for a type which is simply the sum of the tuples
+   of the input types of the functions.
+
+   For instance, for even and odd we have:
+   {[
+     even___fuel : num -> int -> bool result
+     odd___fuel  : num -> int -> bool result
+   ]}
+
+   So the type would be:
+   {[
+     (num # int) + (num # int)
+   ]}
+
+   Note that generally speaking we expect a type of the shape (the “:num”
+   on the left is for the fuel):
+   {[
+     (num # ...) + (num # ...) + ... + (num # ...)
+   ]}
+
+   The decreasing measure is simply given by a function which matches over
+   its argument to return the fuel, whatever the case.
+ *)
+fun mk_termination_measure_from_ty (ty : hol_type) : term =
+  let
+    val dtys = map pairSyntax.strip_prod (sumSyntax.strip_sum ty)
+    (* For every tuple, create a match to extract the num *)
+    fun mk_case_of_tuple (tys : hol_type list) : (term * term) =
+      case tys of
+        [] => failwith "mk_termination_measure_from_ty: empty list of types"
+      | [num_ty] =>
+        (* No need for a case *)
+        let val var = genvar num_ty in (var, var) end
+      | num_ty :: rem_tys =>
+        let
+          val scrut_var = genvar (pairSyntax.list_mk_prod tys)
+          val var = genvar num_ty
+          val rem_var = genvar (pairSyntax.list_mk_prod rem_tys)
+          val pats = [(pairSyntax.mk_pair (var, rem_var), var)]
+          val case_tm = TypeBase.mk_case (scrut_var, pats)
+        in
+          (scrut_var, case_tm)
+        end
+     val tuple_cases = map mk_case_of_tuple dtys
+
+    (* For every sum, create a match to extract one of the tuples *)
+    fun mk_sum_case ((tuple_var, tuple_case), (nvar, case_end)) =
+      let
+        val left_pat = sumSyntax.mk_inl (tuple_var, type_of nvar)
+        val right_pat = sumSyntax.mk_inr (nvar, type_of tuple_var)
+        val scrut = genvar (sumSyntax.mk_sum (type_of tuple_var, type_of nvar))
+        val pats = [(left_pat, tuple_case), (right_pat, case_end)]
+        val case_tm = TypeBase.mk_case (scrut, pats)
+      in
+        (scrut, case_tm)
+      end
+    val tuple_cases = rev tuple_cases
+    val (nvar, case_end) = hd tuple_cases
+    val tuple_cases = tl tuple_cases
+    val (scrut, case_tm) = foldl mk_sum_case (nvar, case_end) tuple_cases
+
+    (* Create the function *)
+    val abs_tm = mk_abs (scrut, case_tm)
+    
+    (* Add the “measure term” *)
+    val tm = inst [alpha_tyvar |-> type_of scrut] measure_tm
+    val tm = mk_comb (tm, abs_tm)
+  in
+    tm
+  end
+
+(*
+val ty = “: (num # 'a) + (num # 'b) + (num # 'c)”
+
+val tys = hd dtys
+val num_ty::rem_tys = tys
+
+val (tuple_var, tuple_case) = hd tuple_cases
+*)
+
 fun mk_fuel_defs (def_tms : term list) : thm =
   let
     (* Retrieve the identifiers.
@@ -116,17 +249,16 @@ fun mk_fuel_defs (def_tms : term list) : thm =
        Ex.: def_tm = “even (n : int) : bool result = if i = 0 then Return T else odd (i - 1))”
        We want to retrive: id = “even”
      *)
-    val app = lhs def_tm
     val ids = map (fst o strip_comb o lhs) def_tms
     (* In the definitions, replace the identifiers by new identifiers which use
        fuel.
 
        Ex.:
        def_fuel_tm = “
-         even_fuel (fuel : nat) (n : int) : result bool =
+         even___fuel (fuel : nat) (n : int) : result bool =
            case fuel of 0 => Diverge
-           | SUC fuel => 
-             if i = 0 then Return T else odd_fuel (i - 1))”
+           | SUC fuel' => 
+             if i = 0 then Return T else odd_fuel fuel' (i - 1))”
      *)
      fun mk_fuel_id (id : term) : term =
        let
@@ -138,16 +270,25 @@ fun mk_fuel_defs (def_tms : term list) : thm =
        in fuel_id end
      val fuel_ids = map mk_fuel_id ids
 
-     val fuel_ids_with_fuel = map (fn id => mk_comb (id, fuel_var)) fuel_ids
+     val fuel_ids_with_fuel0 = map (fn id => mk_comb (id, fuel_var0)) fuel_ids
+     val fuel_ids_with_fuel1 = map (fn id => mk_comb (id, fuel_var1)) fuel_ids
 
      (* Recurse through the terms and replace the calls *)
-     val rwr_thms = map (ASSUME o mk_eq) (zip ids fuel_ids_with_fuel)
-     val fuel_tms = map (rhs o concl o (PURE_REWRITE_CONV rwr_thms)) def_tms
+     val rwr_thms0 = map (ASSUME o mk_eq) (zip ids fuel_ids_with_fuel0)
+     val rwr_thms1 = map (ASSUME o mk_eq) (zip ids fuel_ids_with_fuel1)
+
+     fun mk_fuel_tm (def_tm : term) : term =
+       let
+         val (tm0, tm1) = dest_eq def_tm
+         val tm0 = (rhs o concl o (PURE_REWRITE_CONV rwr_thms0)) tm0
+         val tm1 = (rhs o concl o (PURE_REWRITE_CONV rwr_thms1)) tm1
+       in mk_eq (tm0, tm1) end
+     val fuel_tms = map mk_fuel_tm def_tms
 
      (* Add the case over the fuel *)
      fun add_fuel_case (tm : term) : term =
        let
-         val (app, body) = dest_eq tm
+         val (f, body) = dest_eq tm
          (* Create the “Diverge” term with the proper type *)
          val body_ty = type_of body
          val return_ty =
@@ -155,18 +296,45 @@ fun mk_fuel_defs (def_tms : term list) : thm =
            | _ => failwith "unexpected"
          val diverge_tm = mk_diverge_tm return_ty
          (* Create the “SUC fuel” term *)
-         val suc_tm = mk_comb (num_suc_tm, fuel_var)
-         val fuel_tm = TypeBase.mk_case (fuel_var, [(num_zero_tm, diverge_tm), (suc_tm, body)])
-       in mk_eq (app, fuel_tm) end
+         val suc_tm = mk_comb (num_suc_tm, fuel_var1)
+         val fuel_tm =
+           TypeBase.mk_case (fuel_var0, [(num_zero_tm, diverge_tm), (suc_tm, body)])
+       in mk_eq (f, fuel_tm) end
      val fuel_tms = map add_fuel_case fuel_tms
 
      (* Define the auxiliary definitions which use fuel *)
      val fuel_defs_conj = list_mk_conj fuel_tms
+     (* The definition name *)
+     val def_name = (fst o dest_var o hd) fuel_ids
+     (* The tactic to prove the termination *)
+     val rty = ref “:bool”
+     fun prove_termination_tac (asms, g) =
+       let
+         val _ = print_term g
+         val r_tm = (fst o dest_exists) g
+         val _ = rty := type_of r_tm
+         val ty = (hd o snd o dest_type) (!rty)
+         val m_tm = mk_termination_measure_from_ty ty
+       in
+         WF_REL_TAC ‘^m_tm’ (asms, g)
+       end
      (* Define the fuel definitions *)
-     val fuel_defs_thm = Define ‘^fuel_defs_conj’
+     (*
+       val temp_def = Hol_defn def_name ‘^fuel_defs_conj’
+       Defn.tgoal temp_def
+     *)
+     val fuel_defs_thm = tDefine def_name ‘^fuel_defs_conj’ prove_termination_tac
    in
      fuel_defs_thm
    end
+
+(*
+val (asms, g) = top_goal ()
+
+val rty = ref “:num”
+val ty = !rty
+(hd o snd o dest_type) ty
+*)
 
 (*
 val (fuel_tms, fuel_defs_thm) = mk_fuel_defs def_tms
@@ -215,7 +383,7 @@ fun case_progress (asms, g) =
     val scrut = (strip_all_cases_get_scrutinee o lhs) g
   in Cases_on ‘^scrut’ (asms, g) end
 
-(* Tactic to prove the fuel monotonicity theorem *)
+(* Tactic to prove the fuel monotonicity theorem - TODO: move below *)
 fun prove_fuel_mono_tac (pred_def_thms : thm list) (fuel_defs_thm : thm) =
   Induct_on ‘^fuel_var0’ >-(
     (* The ___P predicates are false: n is 0 *)
@@ -269,8 +437,6 @@ fun prove_fuel_mono (pred_def_thms : thm list) (fuel_defs_thm : thm) : thm =
      val fuel_eq_tms = map mk_fuel_eq_tm pred_fuel_tms
      (* Create the conjunction *)
      val fuel_eq_tms = list_mk_conj fuel_eq_tms
-(*     (* Add the “n <= m ==> ...” implication *)
-     val fuel_eq_tms = mk_imp (fuel_vars_le, fuel_eq_tms) *)
      (* Qantify over the fuels *)
      val fuel_eq_tms = list_mk_forall ([fuel_var0, fuel_var1], fuel_eq_tms)
    in
@@ -587,6 +753,7 @@ val expand_defs = gen_expand_defs def_tms
    
  *)
 fun mk_termination_diverge_tms
+  (def_tms : term list)
   (pred_def_thms : thm list)
   (raw_def_thms : thm list)
   (expand_defs : thm list) :
@@ -694,7 +861,7 @@ fun prove_termination_thms
         (* Add the implication *)
         val tm = mk_imp (pred_tm, tm)
         (* Quantify *)
-        val (_, args) = strip_comb fun_tm
+        val (_, args) = strip_comb (lhs fun_eq_tm)
         val tm = list_mk_forall (args, tm)
 
         (* Prove *)
@@ -838,7 +1005,7 @@ fun prove_divergence_thms
         val tm = list_mk_imp ([pred_tm, pred_suc_tm], tm)
 
         (* Quantify *)
-        val (_, args) = strip_comb fun_tm
+        val (_, args) = strip_comb (lhs fun_eq_tm)
         val tm = list_mk_forall (args, tm)
 
         (* Prove *)
@@ -888,3 +1055,154 @@ set_goal ([], tm)
 
 val (asms, g) = top_goal ()
 *)
+
+(* Prove the final lemmas:
+
+   {[
+     !i. even i = even___expand even odd i
+   ]}
+
+   Note that the shape of the theorem is very precise: this helps for the proof.
+   Also, by correctly ordering the assumptions, we make sure that by rewriting
+   we don't convert one of the two to “T”.
+ *)
+fun prove_final_eqs
+  (term_div_tms : (term * term) list)
+  (termination_thms : thm list)
+  (divergence_thms : thm list)
+  (raw_def_thms : thm list)
+  : thm list =
+  let
+    fun prove_one ((pred_tm, fun_eq_tm), (termination_thm, divergence_thm)) : thm =
+      let
+        val (_, args) = strip_comb (lhs fun_eq_tm)
+        val g = list_mk_forall (args, fun_eq_tm)
+        (* We make a case disjunction of the subgoal: “exists n. even___P i n” *)
+        val exists_g = (rhs o concl) (PURE_REWRITE_CONV raw_def_thms (lhs fun_eq_tm))
+        val (_, exists_g, _) = TypeBase.dest_case exists_g
+        val prove_tac =
+          rpt gen_tac >>
+          Cases_on ‘^exists_g’
+          >-( (* Termination *)
+             irule termination_thm >> pure_asm_rewrite_tac [])
+          (* Divergence *)
+          >> irule divergence_thm >> fs []
+          
+      in
+        save_goal_and_prove (g, prove_tac)
+      end    
+  in
+    map prove_one (zip term_div_tms (zip termination_thms divergence_thms))
+  end
+
+(*
+val termination_thm = hd termination_thms
+val divergence_thm = hd divergence_thms
+set_goal ([], g)
+*)
+
+(* The final function: define potentially diverging functions in an error monad *)
+fun DefineDiv (def_qt : term quotation) =
+  let
+    (* Parse the definitions.
+    
+       Example:
+       {[
+         (even (i : int) : bool result = if i = 0 then Return T else odd (i - 1)) /\
+         (odd (i : int) : bool result = if i = 0 then Return F else even (i - 1))
+       ]}
+     *)
+    val def_tms = (strip_conj o list_mk_conj o rev) (Defn.parse_quote def_qt)
+
+    (* Generate definitions which use some fuel
+    
+       Example:
+       {[
+         even___fuel n i =
+           case fuel of
+             0 => Diverge
+           | SUC fuel => 
+             if i = 0 then Return T else odd_fuel (i - 1))
+       ]}
+     *)
+     (* TODO: list of theorems *)
+     val fuel_defs_thm = mk_fuel_defs def_tms
+
+     (* Generate the predicate definitions.
+     
+        {[ even___P n i = = ~is_diverge (even___fuel n i) ]}
+      *)
+     val fuel_def_tms = map (snd o strip_forall) ((strip_conj o concl) fuel_defs_thm)
+     val pred_def_thms = map mk_fuel_predicate_defs (zip def_tms fuel_def_tms)
+     
+     (* Prove the monotonicity property for the fuel, all at once
+
+      *)
+     val fuel_mono_thm = prove_fuel_mono pred_def_thms fuel_defs_thm
+     
+     (* Prove the individual fuel functions - TODO: update
+
+        {[
+          !n i. $LEAST (even___P i) <= n ==> even___fuel n i = even___fuel ($LEAST (even___P i)) i
+        ]}
+      *)
+     val least_fuel_mono_thms = prove_least_fuel_mono pred_def_thms fuel_mono_thm
+
+     (*
+       {[
+         !n i. even___P i n ==> $LEAST (even___P i) <= n
+       ]}
+      *)
+     val least_pred_thms = prove_least_pred_thms pred_def_thms
+
+     (*
+       {[
+         !n i. even___P i n ==> even___P i ($LEAST (even___P i))
+       ]}
+      *)
+     val pred_n_imp_pred_least_thms = prove_pred_n_imp_pred_least_thms pred_def_thms
+
+     (*
+       "Raw" definitions:
+
+       {[
+         even i = if (?n. even___P i n) then even___P ($LEAST (even___P i)) i else Diverge
+       ]}
+      *)
+     val raw_def_thms = define_raw_defs def_tms pred_def_thms fuel_defs_thm
+
+     (*
+       !n i. even___P i n ==> even___fuel n i = even i
+      *)
+     val pred_imp_fuel_eq_raw_def_thms =
+       prove_pred_imp_fuel_eq_raw_def_thms
+         pred_def_thms fuel_def_tms least_fuel_mono_thms
+         least_pred_thms pred_n_imp_pred_least_thms raw_def_thms
+
+     (* "Expand" definitions *)
+     val expand_defs = gen_expand_defs def_tms
+
+     (* Small utility *)
+     val term_div_tms = mk_termination_diverge_tms def_tms pred_def_thms raw_def_thms expand_defs
+
+     (* Termination theorems *)
+     val termination_thms =
+       prove_termination_thms term_div_tms fuel_defs_thm pred_def_thms
+         raw_def_thms expand_defs pred_n_imp_pred_least_thms pred_imp_fuel_eq_raw_def_thms
+
+     (* Divergence theorems *)
+     val divergence_thms =
+       prove_divergence_thms term_div_tms fuel_defs_thm pred_def_thms raw_def_thms expand_defs
+
+     (* Final theorems:
+
+        {[
+          ∀i. even i = even___E even odd i,
+          ⊢ ∀i. odd i = odd___E even odd i
+        ]}
+      *)
+     val final_eqs = prove_final_eqs term_div_tms termination_thms divergence_thms raw_def_thms
+  in
+    (* We return the final equations, which act as rewriting theorems *)
+    final_eqs
+  end
